fragments.v
@@ -1,62 +1,6 @@
-From Coq Require Import Arith.Arith.
-From Coq Require Import Arith.EqNat.
 From Coq Require Import Init.Nat.
 From Coq Require Import Lia.
 From Coq Require Import Lists.List. Import ListNotations.
-
-Definition relation (X : Type) := X -> X -> Prop.
-
-Definition deterministic {X : Type} (R : relation X) :=
-  forall x y1 y2 : X, R x y1 -> R x y2 -> y1 = y2.
-
-Definition normal_form {X : Type}
-              (R : relation X) (t : X) : Prop :=
-  ~ exists t', R t t'.
-
-
-Inductive multi {X : Type} (R : relation X) : relation X :=
-  | multi_refl : forall (x : X), multi R x x
-  | multi_step : forall (x y z : X),
-                    R x y ->
-                    multi R y z ->
-                    multi R x z.
-
-
-Theorem multi_R : forall (X : Type) (R : relation X) (x y : X),
-    R x y -> (multi R) x y.
-Proof.
-  intros X R x y H.
-  apply multi_step with y.
-  - apply H.
-  - apply multi_refl.
-Qed.
-
-Theorem multi_trans :
-  forall (X : Type) (R : relation X) (x y z : X),
-      multi R x y  ->
-      multi R y z ->
-      multi R x z.
-Proof.
-  intros X R x y z G H.
-  induction G.
-    - (* multi_refl *) assumption.
-    - (* multi_step *)
-      apply multi_step with y.
-      + assumption.
-      + apply IHG. assumption.
-Qed.
-
-
-Tactic Notation "print_goal" :=
-  match goal with |- ?x => idtac x end.
-
-Tactic Notation "normalize" :=
-  repeat (print_goal; eapply multi_step ;
-            [ (eauto 10; fail) | simpl]);
-  apply multi_refl.
-
-Definition deterministic {X : Type} (R : relation X) :=
-  forall x y1 y2 : X, R x y1 -> R x y2 -> y1 = y2.
 
 Ltac solve_by_inverts n :=
   match goal with | H : ?T |- _ =>
@@ -69,86 +13,12 @@ Ltac solve_by_inverts n :=
 Ltac solve_by_invert :=
   solve_by_inverts 1.
 
-Definition normal_form {X : Type}
-              (R : relation X) (t : X) : Prop :=
-  ~ exists t', R t t'.
-
 Lemma value_is_nf : forall v,
   value v -> normal_form step v.
 Lemma nf_is_value : forall t,
   normal_form step t -> value t.
 
-Inductive multi {X : Type} (R : relation X) : relation X :=
-  | multi_refl : forall (x : X), multi R x x
-  | multi_step : forall (x y z : X),
-                    R x y ->
-                    multi R y z ->
-                    multi R x z.
-Theorem multi_R : forall (X : Type) (R : relation X) (x y : X),
-    R x y -> (multi R) x y.
-Proof.
-  intros X R x y H.
-  apply multi_step with y.
-  - apply H.
-  - apply multi_refl.
-Qed.
-
-Theorem multi_trans :
-  forall (X : Type) (R : relation X) (x y z : X),
-      multi R x y  ->
-      multi R y z ->
-      multi R x z.
-Proof.
-  intros X R x y z G H.
-  induction G.
-    -  assumption.
-    -
-      apply multi_step with y.
-      + assumption.
-      + apply IHG. assumption.
-Qed.
-
-Definition step_normal_form := normal_form step.
-
-Definition normal_form_of (t t' : tm) :=
-  (t -->* t' /\ step_normal_form t').
-
-Theorem normal_forms_unique:
-  deterministic normal_form_of.
-Definition normalizing {X : Type} (R : relation X) :=
-  forall t, exists t',
-    (multi R) t t' /\ normal_form R t'.
-
-Tactic Notation "normalize" :=
-  repeat (print_goal; eapply multi_step ;
-            [ (eauto 10; fail) | simpl]);
-  apply multi_refl.
-
-Notation step_normal_form := (normal_form step).
-
-Definition stuck (t : tm) : Prop :=
-  step_normal_form t /\ ~ value t.
-
-Hint Unfold stuck : core.
-
-Definition nf : tm -> Prop := normal_form step.
-
-Theorem nf_if_value (t : tm) : value t -> nf t.
-
-Ltac find_value_step :=
-  match goal with
-  Hv : value ?t,
-  Hs : ?t --> ?t'
-  |- _ => exfalso; apply (nf_if_value t Hv (ex_intro _ t' Hs)) end.
-
-Ltac find_value_step_aggr :=
-  match goal with
-  Hs : ?t --> ?t'
-  |- _ => exfalso; assert (Hv : value t); [eauto | apply (nf_if_value t Hv (ex_intro _ t' Hs))] end.
-
 Theorem type_unique t : forall Gamma T1 T2, Gamma |-- t \in T1 -> Gamma |-- t \in T2 -> T1 = T2.
-
-Definition normalizing (t : tm) := exists t', t -->* t' /\ nf t'.
 
 Definition context_value := list (string * tm * ty).
 
@@ -170,26 +40,3 @@ Ltac get_value :=
   |- _ =>
   let HT' := fresh"HT" in assert (HT' := multi_pre _ _ _ H3 H2); clear H2;
   let Hv := fresh"Hv" in assert (Hv := value_if_nf_ty _ _ HT' H1); clear H1 end.
-
-
-Useful self-defined tactics:
-	in deterministic, find value -> _ and inverse.
-	in deterministic,
-Ltac find_contra :=
-  match goal with
-    H1: ?E = true,
-    H2: ?E = false
-    |- _ => congruence
-  end.
-Ltac clear_refl_eq :=
-  match goal with
-    H1: ?E = ?E
-    |- _ => clear H1
-  end.
-Ltac spec_des :=
-  match goal with
-    H1 : forall (res : result) (st : state), ?P res st -> _,
-    H2 : ?P ?st1 ?res1,
-    H3 : ?P ?st0 ?res0
-    |- _ => destruct (H1 _ _ H2); destruct (H1 _ _ H3); clear H1; repeat clear_refl_eq
-  end.
